Equations version of retyping (principal types theorem is a corrolary)

safechecker/theories/PCUICSafeRetyping.v
@@ -1,17 +1,38 @@
 (* Distributed under the terms of the MIT license. *)
-From MetaCoq.Template Require Import config utils uGraph.
+
+Require Import Equations.Prop.DepElim.
+From Equations Require Import Equations.
+
+From Coq Require Import Bool String List Program.
+From MetaCoq.Template Require Import config monad_utils utils uGraph.
 From MetaCoq.PCUIC Require Import PCUICAst PCUICInduction PCUICLiftSubst
-     PCUICUnivSubst PCUICTyping PCUICSafeLemmata PCUICValidity.
+     PCUICUnivSubst PCUICTyping PCUICSafeLemmata PCUICSubstitution PCUICValidity
+     PCUICGeneration PCUICInversion PCUICValidity PCUICInductives PCUICSR
+     PCUICCumulativity PCUICConversion PCUICConfluence PCUICArities
+     PCUICWeakeningEnv.
 From MetaCoq.SafeChecker Require Import PCUICSafeReduce PCUICSafeChecker.
 
-(** * Retyping
+Require Import ssreflect.
 
-  The [type_of] function provides a fast (and loose) type inference
-  function which assumes that the provided term is already well-typed in
-  the given context and recomputes its type. Only reduction (for
-  head-reducing types to uncover dependent products or inductives) and
-  substitution are costly here. No universe checking or conversion is done
-  in particular. *)
+
+Require Import PCUICAstUtils.
+Lemma cumul_Ind_Ind_inv {cf:checker_flags} {Σ : global_env_ext} Γ ind u args ind' u' args' : 
+  wf Σ ->
+  Σ ;;; Γ |- mkApps (tInd ind u) args <= mkApps (tInd ind' u') args' ->
+  eq_inductive ind ind' *
+  PCUICEquality.R_global_instance Σ (eq_universe Σ) (leq_universe Σ) (IndRef ind) #|args| u u' *
+  All2 (conv Σ Γ) args args'.
+Proof.
+  intros wfΣ cum.
+  eapply invert_cumul_ind_l in cum as [ui' [l' [redl [ru conv]]]]; auto.
+  eapply red_mkApps_tInd in redl as [args'' [eqind red']]; auto.
+  apply mkApps_eq_inj in eqind as [eq ->]=> //; auto. noconf eq.
+  intuition auto.
+  eapply eq_inductive_refl.
+  transitivity args''; auto.
+  eapply All2_symmetry. typeclasses eauto.
+  eapply (All2_impl red'). intros x y; apply red_conv.
+Qed.
 
 
 Derive NoConfusion for type_error.
@@ -19,6 +40,29 @@ Derive NoConfusion for type_error.
 Set Equations With UIP.
 
 Add Search Blacklist "_graph_mut".
+
+Notation ret t := (exist t _).
+
+Definition well_sorted {cf:checker_flags} Σ Γ T := 
+  ∥ ∑ s, Σ ;;; Γ |- T : tSort s ∥.
+
+
+(** * Retyping
+
+  The [infer] function provides a fast (and loose) type inference
+  function which assumes that the provided term is already well-typed in
+  the given context and recomputes its type. Only reduction (for
+  head-reducing types to uncover dependent products or inductives) and
+  substitution are costly here. No universe checking or conversion is done
+  in particular. *)
+
+Definition principal_type {cf:checker_flags} Σ Γ t := { T : term | ∥ (Σ ;;; Γ |- t : T) * (forall T', Σ ;;; Γ |- t : T' -> Σ ;;; Γ |- T <= T') ∥ }.
+Definition principal_sort {cf:checker_flags} Σ Γ T := { s : Universe.t | ∥ (Σ ;;; Γ |- T : tSort s) * (forall s', Σ ;;; Γ |- T : tSort s' -> leq_universe Σ s s') ∥ }.
+
+Definition principal_typed_type {cf:checker_flags} {Σ Γ t} (wt : principal_type Σ Γ t) := proj1_sig wt.
+Definition principal_sort_sort {cf:checker_flags} Σ Γ T (ps : principal_sort Σ Γ T) : Universe.t := proj1_sig ps.
+Coercion principal_typed_type : principal_type >-> term.
+Coercion principal_sort_sort : principal_sort >-> Universe.t.
 
 Section TypeOf.
   Context {cf : checker_flags}.
@@ -33,278 +77,492 @@ Section TypeOf.
     apply validity in H; auto. destruct H as [wfA | [s tyT]].
     right. constructor. auto. left. econstructor; eauto.
   Qed.
+End TypeOf.
 
+Lemma reduce_to_ind_complete {cf:checker_flags} {Σ : global_env_ext} (wfΣ : wf Σ) Γ ty wat e : 
+  reduce_to_ind (sq wfΣ) Γ ty wat = TypeError e ->  
+  (∑ ind u args, red Σ Γ ty (mkApps (tInd ind u) args)) -> False.
+Proof.
+Admitted.
+
+Section TypeOf.
+  Context {cf : checker_flags}.
+  Context (Σ : global_env_ext).
+  Context (hΣ : ∥ wf Σ ∥) (Hφ : ∥ on_udecl Σ.1 Σ.2 ∥).
+  Context (G : universes_graph) (HG : is_graph_of_uctx G (global_ext_uctx Σ)).
 
   Section SortOf.
-    Context (type_of : forall Γ t, welltyped Σ Γ t -> typing_result (∑ T, ∥ Σ ;;; Γ |- t : T ∥)).
-
-    Program Definition type_of_as_sort Γ t (wf : welltyped Σ Γ t) : typing_result Universe.t :=
-      tx <- type_of Γ t wf ;;
-      wfs <- @reduce_to_sort cf Σ hΣ Γ (projT1 tx) _ ;;
-      ret (m:=typing_result) (projT1 wfs).
-    Next Obligation. destruct X. now eapply typing_wellformed. Qed.
-
+    Obligation Tactic := idtac.
+    Program Definition infer_as_sort {Γ t} (wf : well_sorted Σ Γ t)
+      (tx : principal_type Σ Γ t) : principal_sort Σ Γ t :=
+      match @reduce_to_sort cf Σ hΣ Γ tx _ with
+      | Checked (u ; _) => u
+      | TypeError e => !
+      end.
+      
+    Next Obligation. intros Γ t [[s Hs]] [ty [[Hty Hp]]]; simpl.
+      eapply typing_wellformed; eauto. Defined.
+    Next Obligation. intros Γ t ws [s [[Hs Hp]]]. simpl in *.
+      unfold infer_as_sort_obligation_1.
+      destruct ws as [[s' Hs']]. 
+      specialize (Hp _ Hs').
+      eapply invert_cumul_sort_r in Hp as [u' [redu' leq]].
+      destruct reduce_to_sort => //.
+      intros u wc [= <-].
+      todo "Needs completeness of reduce_to_sort"%string.
+    Qed.
+    Next Obligation.
+      simpl. intros.
+      todo "sort"%string.
+    Qed.
   End SortOf.
 
-  Program Definition option_or {A} (a : option A) (e : type_error) : typing_result (∑ x : A, a = Some x) :=
-    match a with
-    | Some d => ret (d; eq_refl)
-    | None => raise e
+  Program Definition infer_as_prod Γ T
+    (isprod : ∥ ∑ na A B, Σ ;;; Γ |- T <= tProd na A B ∥) : 
+    ∑ na' A' B', ∥ red Σ.1 Γ T (tProd na' A' B') ∥ :=
+    match @reduce_to_prod cf Σ hΣ Γ T _ with
+    | Checked p => p
+    | TypeError e => !
     end.
-
-  Program Fixpoint type_of (Γ : context) (t : term) : welltyped Σ Γ t ->
-                                                      typing_result (∑ T : term, ∥ Σ ;;; Γ |- t : T ∥) :=
-    match t return welltyped Σ Γ t -> typing_result (∑ T : term, ∥ Σ ;;; Γ |- t : T ∥) with
-    | tRel n => fun wf =>
-                  t <- option_or (option_map (lift0 (S n) ∘ decl_type) (nth_error Γ n)) (UnboundRel n);;
-                  ret (t.π1; _)
-
-    | tVar n => fun wf => raise (UnboundVar n)
-    | tEvar ev args => fun wf => raise (UnboundEvar ev)
-
-    | tSort s => fun wf => ret (tSort (Universe.try_suc s); _)
-
-    | tProd n t b => fun wf =>
-      s1 <- type_of_as_sort type_of Γ t _ ;;
-      s2 <- type_of_as_sort type_of (Γ ,, vass n t) b _ ;;
-      ret (tSort (Universe.sort_of_product s1 s2); _)
-
-    | tLambda n t b => fun wf =>
-      t2 <- type_of (Γ ,, vass n t) b _;;
-      ret (tProd n t t2.π1; _)
-
-    | tLetIn n b b_ty b' => fun wf =>
-      b'_ty <- type_of (Γ ,, vdef n b b_ty) b' _ ;;
-      ret (tLetIn n b b_ty b'_ty.π1; _)
-
-    | tApp t a => fun wf =>
-      ty <- type_of Γ t _ ;;
-      pi <- reduce_to_prod hΣ Γ ty.π1 _ ;;
-      ret (subst10 a pi.π2.π2.π1; _)
-
-    | tConst cst u => fun wf =>
-          match lookup_env (fst Σ) cst with
-          | Some (ConstantDecl d) =>
-            let ty := subst_instance_constr u d.(cst_type) in
-            ret (ty; _)
-          |  _ => raise (UndeclaredConstant cst)
-          end
-
-    | tInd ind u => fun wf =>
-          d <- @lookup_ind_decl Σ ind ;;
-          let ty := subst_instance_constr u d.π2.π1.(ind_type) in
-          ret (ty; _)
-
-    | tConstruct ind k u => fun wf =>
-          d <- @lookup_ind_decl Σ ind ;;
-          match nth_error d.π2.π1.(ind_ctors) k with
-          | Some cdecl =>
-            ret (type_of_constructor d.π1 cdecl (ind, k) u; _)
-          | None => raise (UndeclaredConstructor ind k)
-          end
-
-    | tCase (ind, par) p c brs => fun wf =>
-      ty <- type_of Γ c _ ;;
-      indargs <- reduce_to_ind hΣ Γ ty.π1 _ ;;
-      ret (mkApps p (List.skipn par indargs.π2.π2.π1 ++ [c]); _)
-
-    | tProj (ind, n, k) c => fun wf =>
-       d <- @lookup_ind_decl Σ ind ;;
-       match nth_error d.π2.π1.(ind_projs) k with
-       | Some pdecl =>
-            c_ty <- type_of Γ c _ ;;
-            indargs <- reduce_to_ind hΣ Γ c_ty.π1 _ ;;
-            let ty := snd pdecl in
-            ret (subst0 (c :: List.rev (indargs.π2.π2.π1)) (subst_instance_constr indargs.π2.π1 ty);
-                   _)
-       | None => !
-       end
-
-    | tFix mfix n => fun wf =>
-      match nth_error mfix n with
-      | Some f => ret (f.(dtype); _)
-      | None => raise (IllFormedFix mfix n)
-      end
-
-    | tCoFix mfix n => fun wf =>
-      match nth_error mfix n with
-      | Some f => ret (f.(dtype); _)
-      | None => raise (IllFormedFix mfix n)
-      end
-    end.
-
+    Next Obligation. exact (todo "completeness"). Qed.
+    Next Obligation. exact (todo "completeness"). Qed.
+  Check !.
+  
+  Equations lookup_ind_decl ind : typing_result
+        ({decl & {body & declared_inductive (fst Σ) decl ind body}}) :=
+  lookup_ind_decl ind with inspect (lookup_env (fst Σ) ind.(inductive_mind)) :=
+    { | exist (Some (InductiveDecl decl)) look with inspect (nth_error decl.(ind_bodies) ind.(inductive_ind)) :=
+      { | exist (Some body) eqnth => Checked (decl; body; _);
+        | ret None => raise (UndeclaredInductive ind) };
+      | _ => raise (UndeclaredInductive ind) }.
   Next Obligation.
-    destruct wf. sq.
-    destruct (nth_error Γ n) eqn:Heq; try discriminate. injection X. intros <-.
-    econstructor; eauto using typing_wf_local.
+    split.
+    - symmetry in look.
+      etransitivity. eassumption. reflexivity.
+    - now symmetry.
   Defined.
 
-  Solve All Obligations with Program.Tactics.program_simpl; try match goal with
-                                              [ |- ∥ _ ∥ ] => todo "PCUICSafeRetyping.type_of"
-                                            | [ |- welltyped _ _ _ ] => todo "PCUICSafeRetyping.type_of"
-                                            | [ |- wellformed _ _ _ ] => todo "PCUICSafeRetyping.type_of"
-                             end.
-  Next Obligation.
-    todo "PCUICSafeRetyping.type_of".
+  Lemma lookup_ind_decl_complete ind e : lookup_ind_decl ind = TypeError e -> 
+    ((∑ mdecl idecl, declared_inductive Σ mdecl ind idecl) -> False).
+  Proof.
+    apply_funelim (lookup_ind_decl ind).
+    1-2:intros * _ her [mdecl [idecl [declm decli]]];
+    red in declm; rewrite declm in e0; congruence.
+    1-2:intros * _ _ => // => _ [mdecl [idecl [declm /= decli]]].
+    red in declm. rewrite declm in e1. noconf e1.
+    congruence.
+  Qed.
+
+  Obligation Tactic := idtac.
+  
+  Local Notation ret t := (exist t _).
+
+  Equations? infer (Γ : context) (t : term) (wt : welltyped Σ Γ t) : principal_type Σ Γ t 
+    by struct t :=
+  { infer Γ (tRel n) wt with 
+    inspect (option_map (lift0 (S n) ∘ decl_type) (nth_error Γ n)) := 
+    { | ret None => !;
+      | ret (Some t) => ret t };
+    
+    infer Γ (tVar n) wt := !;
+    infer Γ (tEvar ev args) wt := !;
+
+    infer Γ (tSort s) _ := ret (tSort (Universe.try_suc s));
+
+    infer Γ (tProd n ty b) wt :=
+      let ty1 := infer Γ ty _ in
+      let s1 := infer_as_sort (todo "wt") ty1 in
+      let ty2 := infer (Γ ,, vass n ty) b _  in
+      let s2 := infer_as_sort (todo "wt2") ty2 in
+      ret (tSort (Universe.sort_of_product s1 s2));
+
+    infer Γ (tLambda n t b) wt :=
+      let t2 := infer (Γ ,, vass n t) b _ in
+      ret (tProd n t t2);
+
+    infer Γ (tLetIn n b b_ty b') wt :=
+      let b'_ty := infer (Γ ,, vdef n b b_ty) b' _ in
+      ret (tLetIn n b b_ty b'_ty);
+
+    infer Γ (tApp t a) wt :=
+      let ty := infer Γ t _ in
+      let pi := infer_as_prod Γ ty _  in
+      ret (subst10 a pi.π2.π2.π1);
+
+    infer Γ (tConst cst u) wt with inspect (lookup_env (fst Σ) cst) :=
+      { | ret (Some (ConstantDecl d)) := ret (subst_instance_constr u d.(cst_type));
+        |  _ := ! };
+
+    infer Γ (tInd ind u) wt with inspect (lookup_ind_decl ind) :=
+      { | ret (Checked decl) := ret (subst_instance_constr u decl.π2.π1.(ind_type));
+        | ret (TypeError e) := ! };
+    
+    infer Γ (tConstruct ind k u) wt with inspect (lookup_ind_decl ind) :=
+      { | ret (Checked d) with inspect (nth_error d.π2.π1.(ind_ctors) k) := 
+        { | ret (Some cdecl) => ret (type_of_constructor d.π1 cdecl (ind, k) u);
+          | ret None => ! };
+      | ret (TypeError e) => ! };
+
+    infer Γ (tCase (ind, par) p c brs) wt with inspect (reduce_to_ind hΣ Γ (infer Γ c _) _) :=
+      { | ret (Checked indargs) =>
+          ret (mkApps p (List.skipn par indargs.π2.π2.π1 ++ [c]));
+        | ret (TypeError _) => ! };
+
+    infer Γ (tProj (ind, n, k) c) wt with inspect (@lookup_ind_decl ind) :=
+      { | ret (Checked d) with inspect (nth_error d.π2.π1.(ind_projs) k) :=
+        { | ret (Some pdecl) with inspect (reduce_to_ind hΣ Γ (infer Γ c _) _) :=
+          { | ret (Checked indargs) => 
+              let ty := snd pdecl in
+              ret (subst0 (c :: List.rev (indargs.π2.π2.π1)) (subst_instance_constr indargs.π2.π1 ty));
+            | ret (TypeError _) => ! };
+         | ret None => ! };
+        | ret (TypeError e) => ! };
+
+    infer Γ (tFix mfix n) wt with inspect (nth_error mfix n) :=
+      { | ret (Some f) => ret f.(dtype);
+        | ret None => ! };
+
+    infer Γ (tCoFix mfix n) wt with inspect (nth_error mfix n) :=
+      { | ret (Some f) => ret f.(dtype);
+        | ret None => ! }
+  }.
+  Proof.
+    all:destruct hΣ, Hφ; destruct wt as [T HT]; try clear infer.
+    all:try solve [econstructor; eauto].
+
+    - sq. destruct (nth_error Γ n) eqn:hnth => //.
+      eapply inversion_Rel in HT as (? & ? & ? & ?); auto.
+      rewrite e in hnth; noconf hnth. noconf wildcard0.
+      split; [now constructor|].
+      intros T' Ht'.
+      eapply inversion_Rel in Ht' as (? & ? & ? & ?); auto.
+      now rewrite e in e0; noconf e0.
+      
+    - eapply inversion_Rel in HT as (? & ? & ? & ?); auto.
+      rewrite e in wildcard => //.
+     
+    - depind HT. eapply IHHT; eauto.
+
+    - depind HT; eapply IHHT; eauto.
+
+    - eapply inversion_Sort in HT as (l & wf & inl & eqs & cum); auto; subst s.
+      sq.
+      split. eapply meta_conv. econstructor; eauto.
+      f_equal; eapply eq_univ''. simpl.
+      unfold UnivExpr.make, Universe.super.
+      destruct (NoPropLevel.of_level l); simpl; auto.
+      destruct t; simpl; auto.
+      intros T' (l' & wf' & inl' & eqs' & cum')%inversion_Sort; auto.
+      eapply Universe.make_inj in eqs'; subst l'.
+      etransitivity; eauto.
+      do 2 constructor.
+      unfold Universe.make, UnivExpr.make, Universe.super.
+      destruct (NoPropLevel.of_level l); simpl; auto;
+      try destruct t; simpl; auto; reflexivity.
+            
+    - eapply inversion_Prod in HT as (? & ? & ? & ? & ?); try econstructor; eauto.
+    - destruct hΣ. destruct Hφ. destruct (inversion_Prod Σ w HT) as (? & ? & ? & ? & ?); try econstructor; eauto.
+    - simpl in *.
+      destruct (inversion_Prod Σ w HT) as (? & ? & ? & ? & ?).
+      subst ty1 ty2.
+      destruct infer_as_sort as [x1 [[Hx1 Hx1p]]]; simpl.
+      destruct infer_as_sort as [x2 [[Hx2 Hx2p]]]; simpl.
+      subst s1 s2; simpl in *. sq.
+      split.
+      * specialize (Hx1p _ t).
+        specialize (Hx2p _ t0).
+        econstructor; eauto.
+      * intros T' Ht'.
+        eapply inversion_Prod in Ht' as (? & ? & ? & ? & ?); auto.
+        etransitivity; eauto. constructor. constructor.
+        eapply leq_universe_product_mon; eauto.
+
+    - eapply inversion_Lambda in HT as (? & ? & ? & ? & ?); try econstructor; eauto.
+    - simpl in t2. destruct (inversion_Lambda Σ w HT) as (? & ? & ? & ? & ?).
+      destruct infer as [bty' [[Hbty pbty]]]; subst t2; simpl in *.
+      sq. split.
+      * econstructor; eauto.
+      * intros T' (? & ? & ? & ? & ?)%inversion_Lambda; auto.
+        specialize (pbty _ t3).
+        transitivity (tProd n t x2); eauto.
+        eapply congr_cumul_prod; auto.
+
+    - eapply inversion_LetIn in HT as (? & ? & ? & ? & ? & ?); auto.
+      eexists; eauto.
+    - simpl in b'_ty.
+      destruct (inversion_LetIn Σ w HT) as (? & ? & ? & ? & ? & ?).
+      destruct infer as [bty' [[Hbty pbty]]]; subst b'_ty; simpl in *.
+      sq; split.
+      * econstructor; eauto.
+      * intros T' (? & ? & ? & ? & ? & ?)%inversion_LetIn; auto.
+        etransitivity; eauto.
+        eapply cumul_LetIn_bo; eauto.
+
+    - eapply inversion_App in HT as (? & ? & ? & ? & ?); try econstructor; eauto.
+    - simpl in ty. destruct inversion_App as (? & ? & ? & ? & ? & ?).
+      destruct infer as [bty' [[Hbty pbty]]]; subst ty; simpl in *.
+      sq. exists x, x0, x1. now eapply pbty.
+      
+    - simpl in *. destruct inversion_App as (? & ? & ? & ? & ? & ?).
+      destruct infer as [tty [[Htty pbty]]]; subst ty; simpl in *.
+      destruct pi as [na' [A' [B' [red]]]].
+      sq. split.
+      * simpl.
+        eapply type_reduction in Htty; eauto.
+        eapply type_App; eauto.
+        specialize (pbty _ t0).
+        assert (Σ ;;; Γ |- tProd na' A' B' <= tProd x x0 x1).
+        eapply cumul_red_l_inv; eauto.
+        eapply cumul_Prod_Prod_inv in X as [Ha _]; auto.
+        eapply type_Cumul; eauto.
+        eapply validity in Htty; auto.
+        eapply isWAT_tProd in Htty; pcuic.
+        eapply conv_cumul. now symmetry.
+      * intros T' (? & ? & ? & ? & ? & ?)%inversion_App; auto.
+        specialize (pbty _ t2). simpl.
+        etransitivity; [|eassumption].
+        assert (Σ ;;; Γ |- tProd na' A' B' <= tProd x2 x3 x4).
+        { eapply cumul_red_l_inv; eauto. }
+        eapply cumul_Prod_Prod_inv in X as [Ha Hb]; auto.
+        eapply (substitution_cumul _ Γ [vass x2 x3] []); eauto.
+        eapply validity in t2; pcuic.
+        eapply isWAT_tProd in t2 as [_ isWAT]; auto.
+        now eapply isWAT_wf_local in isWAT. pcuic.
+        constructor. constructor.
+        now rewrite subst_empty.
+
+    - eapply inversion_Const in HT as [decl ?] => //.
+      intuition auto. red in a0. rewrite a0 in wildcard. noconf wildcard.
+      sq. split.
+      * constructor; eauto.
+      * intros T' [decl [wf [lookup [cu cum]]]]%inversion_Const; auto.
+        red in lookup. congruence.
+    - apply inversion_Const in HT as [decl [wf [lookup [cu cum]]]]; auto.
+      red in lookup. subst wildcard0. rewrite lookup in e. congruence.
+    - apply inversion_Const in HT as [decl [wf [lookup [cu cum]]]]; auto.
+      red in lookup. subst wildcard0. rewrite lookup in e. congruence.
+
+    - destruct decl as [decl [body decli]].
+      eapply inversion_Ind in HT; auto.
+      dependent elimination HT as [(mdecl; idecl; (wf'', (decli', (rest, cum))))].
+      pose proof (declared_inductive_inj decli decli') as [-> ->].
+      sq. split.
+      * econstructor; eauto.
+      * intros T' HT'.
+        eapply inversion_Ind in HT'; auto.
+        dependent elimination HT' as [(mdecl'; idecl'; (wf''', (decli'', (rest', cum'))))].
+        simpl.
+        now destruct (declared_inductive_inj decli decli'') as [-> ->].
+    - eapply inversion_Ind in HT; auto.
+      dependent elimination HT as [(mdecl; idecl; (wf'', (decli', (rest, cum))))].
+      move: wildcard0. destruct decli' as [look hnth].
+      move=> looki.
+      eapply lookup_ind_decl_complete. now symmetry.
+      exists mdecl, idecl. split; auto.
+
+    - destruct d as [decl [body decli]].
+      assert (declared_constructor Σ decl body (ind, k) cdecl) as declc.
+      { red; intuition auto. }
+      eapply inversion_Construct in HT; auto.
+      dependent elimination HT as [(mdecl; idecl; cdecl; (wf'', (declc', (rest, cum))))].
+      pose proof (declared_constructor_inj declc declc') as [-> [-> ->]].
+      sq. split.
+      * econstructor; eauto.
+      * intros T' HT'.
+        eapply inversion_Construct in HT'; auto.
+        dependent elimination HT' as [(mdecl'; idecl'; cdecl'; (wf''', (declc'', (rest', cum'))))].
+        simpl.
+        now destruct (declared_constructor_inj declc declc'') as [-> [-> ->]].
+    - eapply inversion_Construct in HT; auto.
+      dependent elimination HT as [(mdecl; idecl; cdecl'; (wf'', (declc'', (rest, cum))))].
+      destruct declc''.
+      destruct d as [decl [body decli]].
+      pose proof (declared_inductive_inj decli H0) as [-> ->]. simpl in *. congruence.
+    
+    - symmetry in wildcard2.
+      eapply inversion_Construct in HT; auto.
+      dependent elimination HT as [(mdecl; idecl; cdecl; (wf'', (declc', (rest, cum))))].
+      eapply lookup_ind_decl_complete in wildcard2; eauto.
+      now destruct declc'.
+    
+    - eapply inversion_Case in HT; auto.
+      destruct HT as (u & args & mdecl & idecl & ps & pty & btys & decli & indp & bcp & Hpty & lebs
+        & isco & Hc & Hbtys & all & cum).
+      eexists; eauto.
+    - simpl. destruct inversion_Case as (u & args & mdecl & idecl & ps & pty & btys & decli & indp & bcp & Hpty & lebs
+        & isco & Hc & Hbtys & all & cum).
+      destruct infer as [cty [[Hty Hp]]]. simpl.
+      eapply validity in Hty.
+      eapply wat_wellformed; auto. sq; auto. auto.
+    - simpl in *. 
+      destruct inversion_Case as (u & args & mdecl & idecl & ps & pty & btys & decli & indp & bcp & Hpty & lebs
+        & isco & Hc & Hbtys & all & cum).
+      destruct infer as [cty [[Hty Hp]]].
+      simpl in wildcard. destruct reduce_to_ind => //.
+      injection wildcard. intros ->. clear wildcard.
+      destruct a as [i [u' [l [red]]]].
+      simpl.
+      eapply type_reduction in Hty; eauto.
+      pose proof (Hp _ Hc).
+      assert (Σ ;;; Γ |- mkApps (tInd i u') l <= mkApps (tInd ind u) args).
+      { eapply cumul_red_l_inv; eauto. }
+      eapply cumul_Ind_Ind_inv in X0 as [[eqi Ru] cl]; auto.
+      sq; split; simpl.
+      * eapply type_Cumul. econstructor. 3:eauto. all:eauto.
+        todo "cumulativity here"%string.
+        eapply conv_cumul.
+        eapply mkApps_conv_args; auto.
+        eapply All2_app. 2:repeat (constructor; auto).
+        eapply All2_skipn. now symmetry in cl.
+      * intros T'' Hc'.
+        eapply inversion_Case in Hc' as (u'' & args' & mdecl' & idecl' & ps' & pty'
+           & btys' & decli' & indp' & bcp' & Hpty' & lebs' & isco' & Hc' & Hbtys' & all' & cum'); auto.
+        etransitivity. simpl in cum'. 2:eassumption.
+        eapply conv_cumul, mkApps_conv_args; auto.
+        eapply All2_app. 2:repeat (constructor; auto).
+        eapply All2_skipn.
+        specialize (Hp _ Hc').
+        assert (Σ ;;; Γ |- mkApps (tInd i u') l <= mkApps (tInd ind u'') args').
+        { eapply cumul_red_l_inv; eauto. }
+        eapply cumul_Ind_Ind_inv in X0 as [[eqi' Ru'] cl']; auto.
+      
+    - simpl in wildcard1.
+      destruct inversion_Case as (u & args & mdecl & idecl & ps & pty & btys & decli & indp & bcp & Hpty & lebs
+        & isco & Hc & Hbtys & all & cum).
+      destruct infer as [cty [[Hty Hp]]]. simpl.
+      destruct validity as [_ i]. simpl in wildcard1.
+      specialize (Hp _ Hc).
+      eapply invert_cumul_ind_r in Hp as [ui' [l' [red [Ru ca]]]]; auto.
+      symmetry in wildcard1; eapply reduce_to_ind_complete in wildcard1 => //.
+      now exists ind, ui', l'.
+
+    - eapply inversion_Proj in HT as (u & mdecl & idecl & pdecl' & args & declp & Hc & Hargs & cum); auto.
+      simpl in cum.
+      eexists; eauto.
+    - simpl; destruct inversion_Proj as (u & mdecl & idecl & pdecl' & args & declp & Hc & Hargs & cum); auto.
+      destruct infer as [cty [[Hc' Hc'']]]. simpl.
+      eapply validity in Hc'; auto.
+      eapply wat_wellformed; auto. sq; auto.
+    - simpl in *. destruct inversion_Proj as (u & mdecl & idecl & pdecl' & args & declp & Hc & Hargs & cum); auto.
+      destruct infer as [cty [[Hc' Hc'']]]. simpl.
+      destruct reduce_to_ind => //. injection wildcard1. intros ->.
+      clear wildcard1.
+      destruct a as [i [u' [l [red]]]]. simpl.
+      simpl in red.
+      eapply type_reduction in Hc'; eauto.
+      pose proof (Hc'' _ Hc).
+      assert (Σ ;;; Γ |- mkApps (tInd i u') l <= mkApps (tInd ind u) args).
+      { eapply cumul_red_l_inv; eauto. }
+      eapply cumul_Ind_Ind_inv in X0 as [[eqi' Ru'] cl']; eauto.
+      destruct d as [decl [body decli]].
+      pose proof (declared_inductive_inj (proj1 declp) decli) as [-> ->].
+      assert (declared_projection Σ mdecl idecl (ind, n, k) pdecl).
+      { red; intuition eauto. simpl. eapply declp. }
+      pose proof (@PCUICReflect.eqb_eq inductive _). apply H0 in eqi'. subst ind.
+      destruct (declared_projection_inj declp H) as [_ [_ ->]].
+      sq. split; auto.
+      * econstructor; eauto. now rewrite (All2_length _ _ cl').
+      * intros.
+        eapply inversion_Proj in X0 as (u'' & mdecl' & idecl' & pdecl'' & args' & 
+            declp' & Hc''' & Hargs' & cum'); auto.
+        simpl in *. subst ty.
+        destruct (declared_projection_inj H declp') as [-> [-> ->]].
+        etransitivity; eauto.
+        specialize (Hc'' _ Hc''').
+        assert (Σ ;;; Γ |- mkApps (tInd i u') l <= mkApps (tInd i u'') args').
+        { eapply cumul_red_l_inv; eauto. }
+        eapply cumul_Ind_Ind_inv in X0 as [[eqi'' Ru''] cl'']; auto.
+        todo "cumulative inductives here"%string.
+
+    - simpl in *.
+      destruct inversion_Proj as (u & mdecl & idecl & pdecl' & args & declp & Hc & Hargs & cum); auto.
+      destruct infer as [cty [[Hc' Hc'']]]. simpl.
+      symmetry in wildcard3.
+      eapply reduce_to_ind_complete in wildcard3; auto.
+      clear wildcard3; simpl. specialize (Hc'' _ Hc).
+      eapply invert_cumul_ind_r in Hc'' as [ui' [l' [red [Rgl Ra]]]]; auto.
+      eexists _, _, _; eauto.      
+
+    - eapply inversion_Proj in HT as (u & mdecl & idecl & pdecl' & args & declp & Hc & Hargs & cum); auto.
+      destruct declp; simpl in *.
+      destruct d as [decl [body decli]].
+      destruct (declared_inductive_inj decli H0) as [-> ->].
+      simpl in *. intuition congruence.
+
+    - eapply inversion_Proj in HT as (u & mdecl & idecl & pdecl' & args & declp & Hc & Hargs & cum); auto.
+      symmetry in wildcard5.
+      eapply lookup_ind_decl_complete in wildcard5; auto.
+      destruct declp. do 2 eexists; eauto.
+    
+    - eapply inversion_Fix in HT as [decl [fg [hnth [htys [hbods [wf cum]]]]]]; auto.
+      sq; split.
+      * econstructor; eauto.
+        eapply nth_error_all in htys; eauto. destruct htys as [s Hs]. pcuic.
+        eapply typing_wf_local; eauto.
+      * intros T' HT'.
+        eapply inversion_Fix in HT' as [decl' [fg' [hnth' [htys' [hbods' [wf' cum']]]]]]; auto.
+        congruence.
+      
+    - now eapply inversion_Fix in HT as [decl [fg [hnth [htys [hbods [wf cum]]]]]]; auto.
+
+  - eapply inversion_CoFix in HT as [decl [fg [hnth [htys [hbods [wf cum]]]]]]; auto.
+    sq; split.
+    * econstructor; eauto.
+      eapply nth_error_all in htys; eauto. destruct htys as [s Hs]. pcuic.
+      eapply typing_wf_local; eauto.
+    * intros T' HT'.
+      eapply inversion_CoFix in HT' as [decl' [fg' [hnth' [htys' [hbods' [wf' cum']]]]]]; auto.
+      congruence.
+    
+  - now eapply inversion_CoFix in HT as [decl [fg [hnth [htys [hbods [wf cum]]]]]]; auto.
   Defined.
 
-  (* Program Definition sort_of (Γ : context) (t : term) (wf : welltyped Σ Γ t) : typing_result universe := *)
-  (*   ty <- type_of Γ t wf;; *)
-  (*   type_of_as_sort type_of Γ ty.π1 _. *)
-  (* Next Obligation. *)
-
-
+  Definition type_of Γ t wt : term := (infer Γ t wt).
+  
   Open Scope type_scope.
-
-  Conjecture cumul_reduce_to_sort : forall {Γ T wf s},
-    reduce_to_sort hΣ Γ T wf = Checked s ->
-    Σ ;;; Γ |- T <= tSort s.π1.
-
-  Conjecture cumul_reduce_to_prod : forall {Γ T wf na A B H},
-    reduce_to_prod hΣ Γ T wf = Checked (na; A; B; H) ->
-    forall n, Σ ;;; Γ |- T <= tProd n A B.
-
-  Conjecture congr_cumul_letin : forall {Γ n a A t n' a' A' t'},
-    Σ ;;; Γ |- a <= a' ->
-    Σ ;;; Γ |- A <= A' ->
-    Σ ;;; Γ ,, vdef n a A' |- t <= t' ->
-    Σ ;;; Γ |- tLetIn n a A t <= tLetIn n' a' A' t'.
-
-  Ltac case_eq_match :=
-    lazymatch goal with
-    | |- context [ match ?t with _ => _ end ] =>
-      case_eq t ; try solve [ intros ; discriminate ]
-    | h : context [ match ?t with _ => _ end ] |- _ =>
-      revert h ;
-      case_eq t ; try solve [ intros ; discriminate ]
-    end.
-
-  Ltac deal_as_sort :=
-    lazymatch goal with
-    | h : type_of_as_sort _ _ _ = _ |- _ =>
-      unfold type_of_as_sort in h ;
-      simpl in h
-    end.
-
-  Ltac deal_reduce_to_sort :=
-    lazymatch goal with
-    | h : reduce_to_sort _ _ _ = Checked _ |- _ =>
-      pose proof (cumul_reduce_to_sort h) ;
-      clear h
-    end.
-
-  Ltac deal_reduce_to_prod :=
-    lazymatch goal with
-    | h : reduce_to_prod _ _ _ = Checked _ |- _ =>
-      let hh := fresh h in
-      pose proof (cumul_reduce_to_prod h) as hh ;
-      clear h ;
-      lazymatch goal with
-      | na : name |- _ => specialize (hh na)
-      | |- _ => specialize (hh nAnon)
-      end
-    end.
-
-  Ltac deal_Checked :=
-    match goal with
-    | h : Checked _ = Checked _ |- _ =>
-      inversion h ; subst ; clear h
-    end.
-
-  Ltac go eq :=
-    simpl in eq ; revert eq ;
-    repeat (case_eq_match ; intros) ;
-    repeat deal_as_sort ;
-    repeat (case_eq_match ; intros) ;
-    repeat deal_Checked ;
-    repeat deal_reduce_to_sort ;
-    repeat deal_reduce_to_prod.
-
-  Ltac one_ih :=
-    lazymatch goal with
-    | h : _ -> _ -> (_ ;;; _ |- ?t : _) * _ |- _ ;;; _ |- ?t : _ =>
-      eapply h
-    | h : _ -> _ -> _ * (_ ;;; _ |- _ <= ?A) |- _ ;;; _ |- _ <= ?A =>
-      eapply h
-    end.
-
-  Ltac ih :=
-    one_ih ; eassumption.
-
-  Ltac cih :=
-    eapply type_Cumul ; [
-      ih
-    | try eassumption
-    | try eassumption
-    ].
-
+  
   Definition map_typing_result {A B} (f : A -> B) (e : typing_result A) : typing_result B :=
     match e with
     | Checked a => Checked (f a)
     | TypeError e => TypeError e
     end.
 
-  Theorem type_of_principal :
-    forall {Γ t B} ,
-      forall (wt : welltyped Σ Γ t) wt',
-      type_of Γ t wt = Checked (B; wt') ->
-      forall A, Σ ;;; Γ |- t : A -> Σ ;;; Γ |- B <= A.
+  Arguments iswelltyped {cf Σ Γ t A}.
+
+  Lemma infer_clause_1_irrel Γ n H wt wt' : infer_clause_1 infer Γ n H wt = infer_clause_1 infer Γ n H wt' :> term.
   Proof.
-    intros Γ t B wt wt' eq. simpl in wt'. revert B wt' eq. simpl in wt.
-    induction t using term_forall_list_ind; intros B wt' eq A wA.
-    - cbn in eq. destruct option_or eqn:Heq.
-      destruct a as [x Hx]. simpl in eq.
-      inversion eq. subst. clear eq. clear Heq.
-  Admitted. (* Just inversion lemmas, as we're inducting on the term *)
+    destruct H as [[b|] eq]; simp infer. simpl. reflexivity. bang.
+  Qed.
 
-  (*     rewrite Hx in Heq. simpl in Heq. rewrite e in Hx. simpl in Hx. noconf Hx. *)
-  (*     + eapply cumul_refl'. *)
-  (*     + simpl in eq. discriminate. *)
-  (*   - cbn in eq. inversion eq. subst. clear eq. *)
-  (*     constructor. red. constructor. simpl. simpl. *)
-  (*     + (* Proving Typeᵢ : Typeᵢ₊₁ shouldn't be hard... *) *)
-  (*       admit. *)
-  (*   - go eq. *)
-  (*     unfold type_of_as_sort. rewrite *)
-  (*     split. *)
-  (*     + econstructor ; try eassumption ; try ih ; try cih. *)
-  (*       (* Again we're missing result on how to type sorts... *) *)
-  (*       left. red. exists [], a. *)
-  (*       unfold app_context; simpl; intuition auto with pcuic. *)
-  (*       eapply typing_wf_local; tea. *)
-  (*       left. red. exists [], a0. unfold app_context; simpl; intuition auto with pcuic. *)
-  (*       eapply typing_wf_local; tea. *)
-  (*     + (* Sorts again *) *)
-  (*       simpl. *)
-  (*       admit. *)
-  (*   - go eq. split. *)
-  (*     + econstructor ; try eassumption ; try ih ; try cih. *)
-  (*     + eapply congr_cumul_prod. *)
-  (*       * eapply conv_alt_refl. reflexivity. *)
-  (*       * ih. *)
-  (*   - go eq. split. *)
-  (*     + econstructor ; try eassumption ; try ih ; try cih. *)
-  (*     + eapply congr_cumul_letin. all: try eapply cumul_refl'. *)
-  (*       ih. *)
-  (*   - go eq. split. *)
-  (*     + econstructor ; try eassumption ; try ih ; try cih. *)
-  (*       all: admit. *)
-  (*     + (* eapply cumul_subst. *) *)
-  (*       admit. *)
-  (*   - simpl in eq. split. *)
-  (*     + admit. *)
-  (*     + admit. *)
-  (*   - admit. *)
-  (*   - admit. *)
-  (*   - admit. *)
-  (*   - admit. *)
-  (*   - admit. *)
-  (*   - admit. *)
-  (*   - split. *)
-  (*     + ih. *)
-  (*     + eapply cumul_trans ; try eassumption. *)
-  (* Admitted. *)
+  (* Lemma infer_irrel {Γ t} (wt wt' : welltyped Σ Γ t) : infer Γ t wt = infer Γ t wt' :> term.
+  Proof.
+    funelim (infer Γ t wt); try solve [simp infer; simpl; try bang; auto].
 
+    simp infer. simpl. f_equal. todo "sorts".
+    simp infer. simpl. f_equal. apply H.
+    simp infer; simpl; f_equal. apply H.
+    simp infer. simpl. todo "prod".
+    simp infer. eapply infer_clause_1_irrel. revert Heqcall. bang.
+  Qed.*)
 
+  Lemma type_of_subtype {Γ t T} (wt : Σ ;;; Γ |- t : T) :
+    ∥ Σ ;;; Γ |- type_of Γ t (iswelltyped wt) <= T ∥.
+  Proof.
+    unfold type_of.
+    destruct infer as [P [[HP Hprinc]]].
+    sq. simpl. now eapply Hprinc.
+  Qed.
+
+  (* Note the careful use of squashing here: the principal type is accessible 
+    computationally but the proof it is principal is squashed (in Prop).
+    One could also easily modify the above function to return non-squashed 
+    principal typing derivations, if there is some use for it. *)
+  Theorem principal_types {Γ t} (wt : welltyped Σ Γ t) : 
+    ∑ P, ∥ forall T, Σ ;;; Γ |- t : T -> (Σ ;;; Γ |- t : P) * (Σ ;;; Γ |- P <= T) ∥.
+  Proof.
+    exists (infer Γ t wt).
+    destruct infer as [T' [[HT' HT]]].
+    sq. intuition eauto.
+  Qed.
 
 End TypeOf.
